add myColoringAlgorithm.v

vfa/myColoringAlgorithm.v
@@ -1,235 +1,220 @@
 From VFA Require Import Color.
-(* Require Import Color. *)
 From VFA Require Import Perm.
+From VFA Require Import my_New_Coloring.
+From VFA Require Import myGraphs.
+
 
 (** * My Coloring *)
 
-Definition colors_available := M.t S.t.
-
-Definition coloring_state := prod coloring colors_available.
-
-Definition coloring_of_state (c_s: coloring_state) : coloring :=
-  fst c_s.
-
-Definition c_a_of_state (c_s: coloring_state) : colors_available :=
-  snd c_s.
-
-Function make_state (c : coloring) (c_a: colors_available) : coloring_state :=
-  pair c c_a.
-
+Definition colors_available := positive ->  S.t.
 
 Definition low_deg (K: nat) (n: node) (adj: nodeset) : bool := S.cardinal adj <? K.
 
-Definition uncolored (f: coloring) (n: node) (adj: nodeset) : bool := match M.find n f with Some c => true | None => false end.
+Fixpoint beq_pos (u v : positive) :=
+  match u, v with
+  | xH, xH => true
+  | xO x, xO y => beq_pos x y
+  | xI x, xI y => beq_pos x y
+  | _, _ => false
+  end.
+
+Definition uncolored (f: Coloring) (n: node) (adj: nodeset) : bool := 
+  beq_pos (f n) 5%positive.
 
 (* Choose any uncolored vertex *)
-Function get_next (g: graph) (f: coloring) : option node :=
+Function get_next (g: graph) (f: Coloring) : option node :=
   S.choose (subset_nodes (uncolored f) g).
-(* 
-Proof. ?
-Defined.
-*)
+
+Definition make_full_colors_available (g: graph) (palette: S.t) : colors_available :=
+  fun _ => palette.
+
+Definition empty_colors_available (g: graph) : colors_available :=
+  fun _ => S.empty.
+
+Open Scope positive.
+
+Definition c_a_update (c_a : colors_available) (n : node) (s : S.t) :=
+  fun x' => if n =? x' then s else c_a x'.
+
+Definition delete_color_from_neighbors(g: graph) (c_a: colors_available) (clr: Coloring) (n: node):
+    colors_available :=
+  let color_n := clr n in
+  S.fold (fun ver c_a_cur => 
+              let old_colorset := c_a_cur ver in
+              let new_colorset := S.remove color_n old_colorset in
+              c_a_update c_a_cur ver new_colorset
+          ) (adj g n) c_a.
+
+Close Scope positive.
+
+Definition every_adj_of_node_has_available_colors 
+  (g:graph) (n:node) (c_a: colors_available) : bool :=
+    let neigh := adj g n in
+    S.fold 
+    (fun n flag => 
+        if length (S.elements (c_a n) ) =? 0
+          then false
+          else flag
+    )
+    (adj g n) true.
+
+Definition list_of_adj_of_node_with_one_color_available 
+    (g:graph) (n: node) (c_a: colors_available) : list node :=
+      let neigh := adj g n in
+      S.fold 
+      (fun n array => if length (S.elements (c_a n) ) =? 1
+        then n:: array 
+        else array
+      )
+      (adj g n) [].
+
+Fixpoint process_just_colored_bfs_fun
+  (dummy : nat) (n: node) (g: graph) (c_a : colors_available) (clr: Coloring) :
+    ( Coloring * colors_available) :=
+      match dummy with
+        | 0 => (EmptyColoring 5, empty_colors_available g)
+        | S dummy' =>
+            let neigh := adj g n in
+            let c_a_new := delete_color_from_neighbors g c_a clr n in
+            let list_of_1_clr_av := list_of_adj_of_node_with_one_color_available g n c_a_new in
+            if (eqb false (every_adj_of_node_has_available_colors g n c_a))
+              then (EmptyColoring 5, empty_colors_available g)
+              else
+                  fold_right
+                    (fun next_n cur_c_s =>
+                      let clr_cur := fst cur_c_s in
+                      let c_a_cur := snd cur_c_s in
+                      let new_color := nth 0 (S.elements (c_a_cur next_n)) 1%positive in
+                      let new_clr_cur := update_coloring clr_cur next_n new_color in
+                      process_just_colored_bfs_fun dummy' next_n g c_a_cur new_clr_cur
+                    )
+                     (clr, c_a_new)
+                      list_of_1_clr_av
+      end.
+
+Open Scope positive.
+Definition palette4: S.t := fold_right S.add S.empty [1; 2; 3; 4].
 
 
-Definition nodes' (g: graph) := Mdomain g.
-
-Function make_full_colors_available (g: graph) (palette: S.t) : colors_available :=
-  M.fold (fun n _ m => M.add n palette m) g (M.empty S.t).
-
-
-Function get_colors_av_of_vertex (n: node) (c_a: colors_available) : S.t :=
-  match M.find n c_a with
-    | Some c => c
-    | None => S.empty
-  end.
-
+Function process_just_colored_bfs (n: node) (g: graph) (c_a : colors_available) (clr: Coloring)
+  : ( Coloring * colors_available)  :=
+  process_just_colored_bfs_fun 100 n g c_a clr.
 (*
-Fuction unfold_option_state (c_s: coloring_state) : coloring_state  :=
-  match c_s with 
-    | Some a => a
-    | None => pair M.Empty M.Empty
+Function select (K: nat) (g: graph) {measure M.cardinal g}: list node :=
+  match S.choose (subset_nodes (low_deg K) g) with
+  | Some n => n :: select K (remove_node n g)
+  | None => nil
   end. *)
 
+Compute S.choose S.empty.
 
-Definition delete_color_from_neighbors(g: graph) (c_s: coloring_state) (n: node) : coloring_state :=
-  match M.find n (coloring_of_state c_s) with
-    | Some cur_color => 
-        S.fold 
-          (fun vertex c_s_now  => 
-                    match M.find vertex (c_a_of_state c_s_now) with
-                      | Some colorset => pair (coloring_of_state c_s_now) (M.add vertex (S.remove cur_color colorset) (c_a_of_state c_s_now))
-                      | None => pair (coloring_of_state c_s_now) (c_a_of_state c_s_now)
-                    end
-          )
-          (adj g n) c_s
-    | None => make_state (M.empty _) (M.empty _)
-  end.
+Close Scope positive.
+Fixpoint do_color
+  (dummy: nat) (g: graph) (clr: Coloring) (c_a: colors_available):
+    ( Coloring * colors_available) :=
+      match dummy with
+        | 0 => (clr, c_a)
+        | S dummy' => 
+            let next_vert_op := get_next g clr in
+            match next_vert_op with
+              | None => (clr, c_a)
+              | Some next_vert =>
+                      S.fold
+                       (fun col pair =>
+                         let clr_cur := fst pair in
+                         let c_a_cur := snd pair in
+                         let new_clr := update_coloring clr_cur next_vert col in
+                         let new_S := S.add col S.empty in
+                         let new_c_a := c_a_update c_a_cur next_vert new_S in
+                         let processed := process_just_colored_bfs next_vert g new_c_a new_clr in
+                         let pr_clr := fst processed in
+                         let pr_c_a := snd processed in
+                         if length (S.elements (pr_c_a 1%positive)) =? 0
+                            then pair
+                            else
+                                let res := do_color dummy' g pr_clr pr_c_a in
+                                if length (S.elements ( (snd res) 1%positive )) =? 0
+                                  then pair
+                                  else res
+                       )
+                       (c_a next_vert) (clr, c_a)
+            end
+      end.
 
+Print do_color.
+(* K3 *)
+Open Scope positive.
 
-Definition delete_color_from_neighbors'(g: graph) (c_a: colors_available) (n: node) 
-                                  (cur_color: node): colors_available :=
-  S.fold 
-    (fun vertex colors_now  => 
-              match M.find vertex colors_now with
-                | Some colorset => M.add vertex (S.remove cur_color colorset) colors_now
-                | None => colors_now
-              end
-    )
-    (adj g n) c_a.
-
-
-Definition every_adj_of_node_has_available_colors (g:graph) (n:node) (c_a: colors_available) : bool :=
-  S.fold 
-  (fun n flag => if length (S.elements ( get_colors_av_of_vertex n c_a) ) =? 0 
-    then false 
-    else flag 
-  )
-  (adj g n) true.
-
-Definition every_adj_of_node_has_available_colors' (g:graph) (n:node) (c_s: coloring_state) : bool :=
-  S.fold 
-  (fun n flag => if length (S.elements ( get_colors_av_of_vertex n (c_a_of_state c_s) ) ) =? 0 
-    then false 
-    else flag 
-  )
-  (adj g n) true.
-
-Definition list_of_adj_of_node_with_one_color_available (g:graph) (n: node) (c_a: colors_available) : list node :=
-  S.fold 
-  (fun n array => if length (S.elements ( get_colors_av_of_vertex n c_a) ) =? 1 
-    then n:: array 
-    else array
-  )
-  (adj g n) [].
-
-Definition list_of_adj_of_node_with_one_color_available' (g:graph) (n: node) (c_s: coloring_state) : list node :=
-  S.fold 
-  (fun n array => if length (S.elements ( get_colors_av_of_vertex n (c_a_of_state c_s) ) ) =? 1 
-    then n:: array 
-    else array
-  )
-  (adj g n) [].
-
-(*
-Function color_vertices_with_one_color_available (g: graph) (n:node) (c_a: colors_available) ()
-*)
-(*
-process_updated_colors_available: if not every_vertex_has_available_colors return None, else Some coloring_state.
-*)
-(*
-Function process_updated_colors_available (g:graph) (n:node) (c: coloring) (c_a: colors_available) : option coloring_state:=
-  if every_adj_of_node_has_available_colors =? false 
-    then None
-    else fold (fun node ) (list_of_adj_of_node_with_one_color_available g n c_a) (pair c c_a).
-
-process_just_colored_bfs: 
-*)
-
-Fixpoint process_just_colored_bfs' (dummy : nat) (n: node) (g: graph) (c_s : coloring_state) : option coloring_state :=  
-  match dummy with
-  | 0 => None
-  | S p =>
-      match every_adj_of_node_has_available_colors' g n (delete_color_from_neighbors g c_s n) with
-      | false => None
-      | true => 
-          fold_right 
-            (fun next_vertice cur_c_s => 
-                  match cur_c_s with
-                    | None => None
-                    | Some c_s_ => process_just_colored_bfs' p next_vertice g c_s_
-                  end
-            ) (Some c_s) (list_of_adj_of_node_with_one_color_available' g n c_s)
-      end
-  end.
-
-(*! FIXME: set dummy parameter to a provably safe value. *)
-
-Function process_just_colored_bfs (n: node) (g: graph) (c_s : coloring_state) : option coloring_state :=
-  process_just_colored_bfs' 100 n g c_s.
+Definition coloring1 := 
+  update_coloring (EmptyColoring 5) 1 1.
 
 
+Definition S1 := fold_right S.add S.empty [1].
 
-(* ################################################################# *)
-(** * Proof of Correctness of the Algorithm. *)
+Definition c_a_1 :=
+  c_a_update (make_full_colors_available K3 palette4) 1 S1.
 
-(** We want to show that any coloring produced by the [color] function actually
-  respects the interference constraints.  This property is called [coloring_ok].  
-*)
 
-Definition coloring_ok (palette: S.t) (g: graph) (f: coloring) :=
- forall i j, S.In j (adj g i) -> 
-     (forall ci, M.find i f = Some ci -> S.In ci palette) /\
-     (forall ci cj, M.find i f = Some ci -> M.find j f = Some cj -> ci<>cj).
+Definition clr_res1 := fst (process_just_colored_bfs 1 K3 c_a_1 coloring1).
+Definition c_a_res1 := snd (process_just_colored_bfs 1 K3 c_a_1 coloring1).
 
-(** **** Exercise: 2 stars (adj_ext)  *)
-Lemma adj_ext: forall g i j, E.eq i j -> S.eq (adj g i) (adj g j).
-(* FILL IN HERE *) Admitted.
-(** [] *)
 
-(** **** Exercise: 3 stars (in_colors_of_1)  *)
-Lemma in_colors_of_1:
-  forall i s f c, S.In i s -> M.find i f = Some c -> S.In c (colors_of f s).
-(* FILL IN HERE *) Admitted.
-(** [] *)
+Definition res := do_color 1 K3 (EmptyColoring 5) (make_full_colors_available K3 palette4).
 
-(** **** Exercise: 4 stars (color_correct)  *)
-Theorem color_correct:
-  forall palette g, 
-       no_selfloop g -> 
-       undirected g -> 
-       coloring_ok palette g (color palette g).
-(* FILL IN HERE *) Admitted.
-(** [] *)
 
-(** That concludes the proof that the algorithm is correct. *)
+Compute (fst res) 1.
+Compute (fst res) 2.
+Compute (fst res) 3.
+
+Compute S.elements ((snd res) 1).
+Compute S.elements ((snd res) 2).
+Compute S.elements ((snd res) 3).
+
+
+Compute S.elements ( (make_full_colors_available K3 palette4) 3).
+
+
+Definition res_clr := fst (do_color 100 K3).
+Compute (fst res) 1.
+Compute (fst res) 2.
+Compute (fst res) 3.
+Definition res_c_a := snd (do_color K3).
+
+Compute do_color 100 K3 
+
+
+Compute res_c_a.
+
+Compute clr_res1 1.
+Compute clr_res1 2.
+Compute clr_res1 3.
+Compute clr_res1 4.
+
+Compute S.elements (c_a_res1 1).
+Compute S.elements (c_a_res1 2).
+Compute S.elements (c_a_res1 3).
+Compute S.elements (c_a_res1 4).
+
+(* process_just_colored_bfs seems to work *)
 
 
 (* ################################################################# *)
 (** * Trying Out the Algorithm on an Actual Test Case *)
 
 Local Open Scope positive.
-(* now 1,2,3, etc. are notation for [positive] numbers. *)
-(* Let's use only three colors *)
-Definition palette: S.t := fold_right S.add S.empty [1; 2; 3].
-
-Definition add_edge (e: (E.t*E.t)) (g: graph) : graph :=
- M.add (fst e) (S.add (snd e) (adj g (fst e))) 
-  (M.add (snd e) (S.add (fst e) (adj g (snd e))) g).
-
-Definition mk_graph (el: list (E.t*E.t)) :=
-  fold_right add_edge (M.empty _) el.
-
-Definition G := 
-    mk_graph [ (5,6); (6,2); (5,2); (1,5); (1,2); (2,4); (1,4)].
-
-Compute (S.elements (Mdomain G)). (* = [4; 2; 6; 1; 5] *)
-
-Compute (M.elements (color palette G)). (* = [(4, 1); (2, 3); (6, 2); (1, 2); (5, 1)] *)
-
-(** That is our graph coloring:  Node [4] is colored with color [1], node [2] with color [3],
-  nodes [6] and [1] with [2], and node [5] with color [1]. *)
-
-(* ################################################################# *)
-(** * Trying Out the My_Coloring  *)
-
 Definition palette4: S.t := fold_right S.add S.empty [1; 2; 3; 4].
 
+Compute (S.elements (Mdomain K3)).
 
-Definition G' := 
-    mk_graph [ (1, 2) ; (2, 3); (1, 3)].
+Compute (M.elements (color palette4 H)).
 
-Compute (S.elements (Mdomain G')). (* = [2; 1; 3] *)
-
-Compute (M.elements (color palette G')).
-
-Definition full_colors4_3 := make_full_colors_available G' palette4.
-
-Check full_colors4_3.
+Definition full_colors4_3 := make_full_colors_available K3 palette4.
+Compute M.elements full_colors4_3.
 
 Compute match (M.find 3 full_colors4_3) with Some c => (S.elements c) | None => nil end.
 (* = [4; 2; 1; 3] -- colors available for vertex 3 in full_colors4_3 *)
 
-Definition delete_color1_from2_3 := delete_color_from_neighbors' G' full_colors4_3 1 1.
+Definition delete_color1_from2_3 := delete_color_from_neighbors G' full_colors4_3 1 1.
 Definition delete_color1_2_from2_3 := delete_color_from_neighbors' G' delete_color1_from2_3 1 2.
 Definition delete_color1_2_3_from2_3 := delete_color_from_neighbors' G' delete_color1_2_from2_3 1 3.
 Definition delete_color1_2_3_4_from2_3 := delete_color_from_neighbors' G' delete_color1_2_3_from2_3 1 4.
